bedrock2/src/bedrock2Examples/swap.v
@@ -20,6 +20,9 @@ Definition swap_swap := let a := "a" in let b := "b" in
   swap(a, b)
 ))).
 
+Definition main :=
+  ("main", ([]: list varname, []: list varname, cmd.call [] "swap_swap" [expr.literal 100; expr.literal 108])).
+
 Require bedrock2.WeakestPrecondition.
 Require Import bedrock2.Semantics bedrock2.FE310CSemantics.
 Require Import coqutil.Map.Interface bedrock2.Map.Separation bedrock2.Map.SeparationLogic.
@@ -38,32 +41,32 @@ Section WithParameters.
       WeakestPrecondition.call (p:=@semantics_parameters p) functions
         "swap" t m [a_addr; b_addr]
         (fun t' m' rets => t=t'/\ (scalar a_addr b * (scalar b_addr a * R)) m' /\ rets = nil).
-  
+
   Instance spec_of_swap_swap : spec_of "swap_swap" := fun functions =>
     forall a_addr a b_addr b m R t,
       (scalar a_addr a * (scalar b_addr b * R)) m ->
       WeakestPrecondition.call (p:=@semantics_parameters p) functions
         "swap_swap" t m [a_addr; b_addr]
         (fun t' m' rets => t=t' /\ (scalar a_addr a * (scalar b_addr b * R)) m' /\ rets = nil).
-  
+
   Require Import bedrock2.string2ident.
-  
+
   Lemma swap_ok : program_logic_goal_for_function! swap.
   Proof.
     repeat straightline; []; eauto.
   Defined.
-  
+
   Lemma swap_swap_ok : program_logic_goal_for_function! swap_swap.
   Proof.
     repeat (straightline || (straightline_call; [solve[SeparationLogic.ecancel_assumption]|])); []; eauto.
   Defined.
-  
+
   Lemma link_swap_swap_swap_swap : spec_of_swap_swap (swap_swap::swap::nil).
   Proof. auto using swap_swap_ok, swap_ok. Qed.
-  
+
   (* Print Assumptions link_swap_swap_swap_swap. *)
   (* SortedList.* SortedListString.* *)
-  
+
   From bedrock2 Require Import ToCString Byte Bytedump.
   Local Open Scope bytedump_scope.
   Goal True.
